feat: align `List/Array/Vector` `flatten` lemmas (#6640)
This PR completes aligning `List`/`Array`/`Vector` lemmas about
`flatten`. `Vector.flatten` was previously missing, and has been added
(for rectangular sizes only). A small number of missing `Option` lemmas
were also need to get the proofs to go through.

src/Init/Data/Vector/Basic.lean
@@ -170,6 +170,10 @@ result is empty. If `stop` is greater than the size of the vector, the size is u
 @[inline] def map (f : α → β) (v : Vector α n) : Vector β n :=
   ⟨v.toArray.map f, by simp⟩
 
+@[inline] def flatten (v : Vector (Vector α n) m) : Vector α (m * n) :=
+  ⟨(v.toArray.map Vector.toArray).flatten,
+    by rcases v; simp_all [Function.comp_def, Array.map_const']⟩
+
 /-- Maps corresponding elements of two vectors of equal size using the function `f`. -/
 @[inline] def zipWith (a : Vector α n) (b : Vector β n) (f : α → β → φ) : Vector φ n :=
   ⟨Array.zipWith a.toArray b.toArray f, by simp⟩
